\subsection{Induction}

\subsubsection*{\textbf{1-10.} \emph{Prove that $\sum_{i=1}^{n}i=\frac{n(n+1)}{2} \;for\; n \geq 0$, by induction.}}

Let $n = 1$. Then
\begin{soleqo}
	&\frac{n(n+1)}{2} = 1 = \sum_{i=1}^{1} i
\end{soleqo}
establishing our base case. We assume that $\exists n \geq 0 \in  \mathbb{N}$  where
\begin{soleqo}
	\sum_{i=1}^{n} i =& \frac{n(n+1)}{2} \;for\; n \leq \;some\; k \in \mathbb{N}
\end{soleqo}
\text{We must show } \\
\begin{soleqo}
	\sum_{i=1}^{n+1} i &= \frac{(n+1)(n+2)}{2}
\end{soleqo}
	\text{We can see that } \\
\begin{soleqo}
	\sum_{i=1}^{n+1} i =& \; (n+1) + \sum_{i=1}^{n} i \\ \\
					   =& \; (n+1) + \frac{n(n+1)}{2} \\ \\
					   =& \; \frac{[2(n+1) + n(n+1)]}{2} \\ \\
					   =& \; \frac{(n+1)(n+2)}{2} \;\;\blacksquare
\end{soleqo}




\subsubsection*{\textbf{1-11.} \emph{Prove that $\sum_{i=1}^{n}i^{2}=\frac{n(n+1)(2n+1)}{6} \;for\; n \geq 0$, by induction.}} 

Let $n = 1$. Then
\begin{soleqo}
	\frac{n(n+1)(2n+1)}{6} = 1 = \sum_{i=1}^{1} i^{2} 
\end{soleqo}
establishing our base case. We assume that $\exists n \geq 0 \in  \mathbb{N}$ where \\
\begin{soleqo}
	\sum_{i=1}^{n} i^{2} = \frac{n(n+1)(2n+1)}{6} \;for\; n \leq \;some\; k \in \mathbb{N}
\end{soleqo}
We must show \\
\begin{soleqo}
	\sum_{i=1}^{n+1}i^{2}=\frac{(n+1)(n+2)(2n+3)}{6}
\end{soleqo}
We can see that \\
\begin{soleqo}
	\sum_{i=1}^{n+1} i^{2} =& \; (n+1)^{2} + \sum_{i=1}^{n} i^2  \\ \\
						   =& \; (n+1)^{2} + \frac{n(n+1)(2n+1)}{6}  \\ \\
						   =& \; \frac{(n+1)[6(n+1) + n(2n+1)]}{6}  \\ \\
						   =& \; \frac{(n+1)[2n^{2} + 7n + 6]}{6}  \\ \\
						   =& \; \frac{(n+1)(n+2)(2n+3)}{6} \;\blacksquare
\end{soleqo}


{\color{pendsol}{} 

\subsubsection*{\textbf{1-12.} \emph{Prove that $\sum_{i=1}^{n}i^{3}=\frac{n^{2}(n+1)^{2}}{4} \;for\; n \geq 0$, by induction}}

\subsubsection*{\textbf{1-13.} \emph{Prove that $\sum_{i=1}^{n}i(i+1)(i+2)=\frac{n(n+1)(n+2)(n+3)}{4}$ }}

\subsubsection*{\textbf{1-14.} \emph{Prove by induction on $n\geq1$ that for every $a\neq1$,  $\sum_{i=0}^{n}a^{i} = \frac{a^{n+1} - 1}{a - 1}$}}

\subsubsection*{\textbf{1-15.} \emph{Prove by induction that for every $n\geq1$,  $\sum_{i=1}^{n}\frac{1}{i(i+1)} = \frac{n}{n+1}$}}

\subsubsection*{\textbf{1-16.} \emph{Prove by induction that $n^{3}+2n$ is divisible by 3 for all $n\geq0$.}}

\subsubsection*{\textbf{1-17.} \emph{Prove by induction that a tree with n vertices has exactly $n-1$ edges.}}

\subsubsection*{\textbf{1-18.} \emph{Prove by mathematical induction that the sum of the cubes of the first n positive integer is equal to the square of the sum of these integers, i.e.
$$\sum_{i=1}^{n}i^{3} = (\sum_{i=1}^{n}i)^{2}$$}}



}












% \textcolor{answer}{
% 	\text{Let $n = 1$, then}
% 	$$\frac{n(n+1)}{2} = 1 = \sum_{i=1}^{1} i$$
% 	\text{establishing our base case. We assume that $\exists n \geq 0 \in  \mathbb{N}$ where}
% 	$$\sum_{i=1}^{n} i = \frac{n(n+1)}{2} \;for\; n \leq \;some\; k \in \mathbb{N}$$
% 	We must show
% 	$$\sum_{i=1}^{n+1} i = \frac{(n+1)(n+2)}{2}$$
% 	We can see that
% 	\begin{align*}
% 	\sum_{i=1}^{n+1} i =& \; (n+1) + \sum_{i=1}^{n} i \\
% 					   =& \; (n+1) + \frac{n(n+1)}{2} \\
% 					   =& \; \frac{[2(n+1) + n(n+1)]}{2} \\
% 					   =& \; \frac{(n+1)(n+2)}{2} \;{\color{black}\blacksquare}
% 	\end{align*}
% }




% \textbf{1-11.} \emph{Prove that $\sum_{i=1}^{n}i^{2}=\frac{n(n+1)(2n+1)}{6} \;for\; n \geq 0$, by induction} \\
% Let $n = 1$. Then
% $$\frac{n(n+1)(2n+1)}{6} = 1 = \sum_{i=1}^{1} i^{2}$$
% establishing our base case. We assume that $\exists n \geq 0 \in  \mathbb{N}$ where
% $$\sum_{i=1}^{n} i^{2} = \frac{n(n+1)(2n+1)}{6} \;for\; n \leq \;some\; k \in \mathbb{N}$$
% We must show
% $$\sum_{i=1}^{n+1}i^{2}=\frac{(n+1)(n+2)(2n+3)}{6}$$
% We can see that
% \begin{align*}
% \sum_{i=1}^{n+1} i^{2} =& \; (n+1)^{2} + \sum_{i=1}^{n} i^2 \\
% 					   =& \; (n+1)^{2} + \frac{n(n+1)(2n+1)}{6} \\
% 					   =& \; \frac{(n+1)[6(n+1) + n(2n+1)]}{6} \\
% 					   =& \; \frac{(n+1)[2n^{2} + 7n + 6]}{6} \\
% 					   =& \; \frac{(n+1)(n+2)(2n+3)}{6} \;\blacksquare
% \end{align*}


% \textbf{1-12.} \emph{Prove that $\sum_{i=1}^{n}i^{3}=\frac{n^{2}(n+1)^{2}}{4} \;for\; n \geq 0$, by induction}  \\

